fix hist_extend_put, and use it to qed ClientHist.Put wrapper

src/program_proof/pav/client_hist.v
@@ -25,7 +25,7 @@ Context `{!heapGS Σ, !pavG Σ}.
 Definition own (ptr : loc) (obj : t) : iProp Σ :=
   "Hcli" ∷ Client.own ptr (Client.mk obj.(γ) obj.(uid) (W64 $ length obj.(pks))
     obj.(ep_valid) obj.(serv) obj.(serv_is_good)) ∗
-  "#Hhist" ∷ is_hist obj.(γ) obj.(uid) obj.(pks) obj.(ep_valid).
+  "#Hhist" ∷ is_hist obj.(γ) obj.(serv).(Server.vrf_pk) obj.(uid) obj.(pks) obj.(ep_valid).
 
 End defs.
 End ClientHist.
@@ -44,15 +44,38 @@ Lemma wp_Client__Put ptr_c c sl_pk d0 (pk : list w8) :
     let new_c := set ClientHist.pks (λ x, (x ++ [(ep, pk)]))
       (set ClientHist.ep_valid (λ _, word.add ep (W64 1)) c) in
     "Hsl_pk" ∷ own_slice_small sl_pk byteT d0 pk ∗
-    "Hown_err" ∷ ClientErr.own ptr_err err c.(Client.serv).(Server.sig_pk) ∗
-    "%Hgenie" ∷ ⌜ c.(Client.serv_is_good) = true → err.(ClientErr.Err) = false ⌝ ∗
+    "Hown_err" ∷ ClientErr.own ptr_err err c.(ClientHist.serv).(Server.sig_pk) ∗
+    "%Hgenie" ∷ ⌜ c.(ClientHist.serv_is_good) = true → err.(ClientErr.Err) = false ⌝ ∗
     "Herr" ∷ (if err.(ClientErr.Err)
       then
         "Hcli" ∷ ClientHist.own ptr_c c
       else
         "Hcli" ∷ ClientHist.own ptr_c new_c)
   }}}.
-Proof. Admitted.
+Proof.
+  iIntros (Φ) "H HΦ". iNamed "H". iNamed "Hcli".
+  destruct c. simpl in *.
+  destruct serv_is_good eqn:Heq_good.
+  - wp_apply (wp_Client__Put_good with "[$Hcli $Hsl_pk //]").
+    iIntros "*". iNamed 1. simpl in *.
+    iApply "HΦ". iFrame. iSplit; [done|].
+    rewrite Herr. iSplit; simpl in *.
+    { rewrite length_app. simpl.
+      replace (W64 (_ + _)%nat) with
+        (word.add (W64 $ length pks) (W64 1)); [|word].
+      iFrame. }
+    iApply (hist_extend_put with "[$Hhist $His_put_post]"); word.
+  - wp_apply (wp_Client__Put with "[$Hcli $Hsl_pk //]").
+    iIntros "*". iNamed 1. simpl in *.
+    iApply "HΦ". iFrame. iSplit; [done|].
+    case_match; [iFrame "∗#"|]. iNamed "Herr".
+    iSplit; simpl in *.
+    { rewrite length_app. simpl.
+      replace (W64 (_ + _)%nat) with
+        (word.add (W64 $ length pks) (W64 1)); [|word].
+      iFrame. }
+    iApply (hist_extend_put with "[$Hhist $His_put_post]"); word.
+Qed.
 
 (* parallel with normal audit is hist_audit_msv. *)
 Lemma logical_audit (ep : w64) ptr_c c :
